theories/OGSD.v
@@ -11,14 +11,35 @@ Definition ogs {I J} (U : uniform_event I J)
         (fun '(j , ks) q => { i : _ & k_rsp U ((u_rsp U q ++ ks) .[i]) })
         (fun '(j , ks) q r => (k_nxt U (projT2 r) , u_rsp U q ++ ks)).
 
+Definition ogs_conf {I} {U : uniform_event I I}
+             (X : I -> Type) (ks : list (kon U)) : Type :=
+  dvec (fun k => forall r : k_rsp U k, X (k_nxt U r)) ks.
+
 Definition ogs_emb {I} {U : uniform_event I I} {X : I -> Type}
-           : forall {i ks}, itree U X i
-           -> dvec (fun k => forall r : k_rsp U k, itree U X (k_nxt U r)) ks
+           : forall {i ks},
+             ogs_conf (itree U X) ks
+           -> itree U X i
            -> itree (ogs U) (X ∘ fst) (i , ks) :=
-  cofix _ogs_emb i ks x c := match (observe x) with
+  cofix _ogs_emb i ks c x := match (observe x) with
     | RetF x => Ret (x : X (fst (i , ks)))
-    | TauF t => Tau (_ogs_emb i ks t c)
+    | TauF t => Tau (_ogs_emb i ks c t)
     | VisF e k => Vis (e : qry (ogs U) (i , ks)) (fun r =>
-                   let c' := d_concat ks (u_rsp U e) c (fun i r => k (i ,& r)) in
-                   _ogs_emb _ _ (d_get _ c' _ _) c')
+                   let c' := d_concat _ _ c (curry2' k) in
+                   _ogs_emb _ _ c' (d_get _ c' _ _))
     end.
+
+From OGS Require Import EqD.
+
+Definition eutt_conf {I} {U : uniform_event I I} {X ks}
+           : ogs_conf (itree U X) ks -> ogs_conf (itree U X) ks -> Prop :=
+  fun c0 c1 => forall i (r : k_rsp U (ks .[i])), d_get ks c0 i r ≈ d_get ks c1 i r.
+
+Theorem ogs_sound {I} {U : uniform_event I I} {X i ks}
+        (c0 c1 : ogs_conf (itree U X) ks) (a b : itree U X i)
+        : ogs_emb c0 a ≈ ogs_emb c1 b -> eutt_conf c0 c1 * (a ≈ b).
+Admitted.
+
+Theorem ogs_complete {I} {U : uniform_event I I} {X i ks}
+        (c0 c1 : ogs_conf (itree U X) ks) (a b : itree U X i)
+        : (a ≈ b) -> eutt_conf c0 c1 -> ogs_emb c0 a ≈ ogs_emb c1 b.
+Admitted.
